meta/UnverifiedCompilation.fst
@@ -2,10 +2,10 @@ module UnverifiedCompilation
 
 open HelperTactics
 
-type open_stlc_term (g:STLC.env) =
+type open_stlc_term (g:STLC.context) =
   (e:STLC.exp & t:STLC.typ & STLC.typing g e t)
 
-type open_stlc_term' (g:STLC.env) (t:STLC.typ) =
+type open_stlc_term' (g:STLC.context) (t:STLC.typ) =
   (e:STLC.exp & STLC.typing g e t)
 
 let rec make_stlc_nat #g (n:nat) : open_stlc_term' g STLC.TNat = 
@@ -15,7 +15,7 @@ let rec make_stlc_nat #g (n:nat) : open_stlc_term' g STLC.TNat =
     let (|_, tyj |) = make_stlc_nat (n-1) in
     (| _, STLC.TySucc tyj |)
 
-let rec unverified_typ_translation
+let rec typ_translation
   (gfs:env)
   (qfs:term)
   : TacP STLC.typ
@@ -28,22 +28,22 @@ let rec unverified_typ_translation
     | _ ->
       let qfs' = norm_term_env gfs [delta] qfs in
       (* avoid infinite loop by checking if axiom *)
-      if tag_of qfs' <> "Tv_FVar" then unverified_typ_translation gfs qfs'
+      if tag_of qfs' <> "Tv_FVar" then typ_translation gfs qfs'
       else fail (fv_to_string fv ^ " not defined")
   end
 
   | Tv_Arrow b c ->  begin
-    let tbv = unverified_typ_translation gfs b.sort in
+    let tbv = typ_translation gfs b.sort in
     match c with
     | C_Total ret -> 
-      let tc = unverified_typ_translation gfs ret in
+      let tc = typ_translation gfs ret in
       STLC.TArr tbv tc
     | _ -> fail ("not a total function type")
   end
   | Tv_Var v -> fail "fvar"
 
   (** erase refinement **)
-  | Tv_Refine b _ -> unverified_typ_translation gfs b.sort
+  | Tv_Refine b _ -> typ_translation gfs b.sort
 
   | Tv_Const c -> fail (print_vconst c)
 
@@ -53,7 +53,7 @@ let rec unverified_typ_translation
   | _ -> fail ("not implemented")
 
 let comp_typ (nm:string) (qfs:term) : dsl_tac_t = fun g ->
-  let typ= unverified_typ_translation g qfs in
+  let typ= typ_translation g qfs in
 
   let qtyp = quote typ in
   type_dynamically g qtyp (`STLC.typ);
@@ -86,15 +86,15 @@ type fs_var =
 | Var  : namedv -> fs_var
 | Bv   : bv -> fs_var
 
-type mapping (g:STLC.env) =
+type mapping (g:STLC.context) =
   fs_var -> depth:nat -> option (x:STLC.var{Some? (g x)})
 
 let extend_env_mapping
-  (gstlc:STLC.env)
+  (gstlc:STLC.context)
   (vars_mapping:mapping gstlc) 
   (b:binder)
   (b_ty:STLC.typ):
-  (gstlc':STLC.env & mapping gstlc') =
+  (gstlc':STLC.context & mapping gstlc') =
   let gstlc' = STLC.extend b_ty gstlc in
   let vars_mapping': mapping gstlc' =
     (fun x n -> match x with 
@@ -103,9 +103,9 @@ let extend_env_mapping
   (| gstlc', vars_mapping' |)
 
 (* CA: keeping track of the type of the term is important for the logical relation *)
-let rec unverified_exp_translation
+let rec exp_translation
   (gfs:env)
-  (gstlc:STLC.env)
+  (gstlc:STLC.context)
   (vars_mapping:mapping gstlc)
   (qfs:term)
   : TacP (open_stlc_term gstlc)
@@ -129,14 +129,14 @@ let rec unverified_exp_translation
               we don't have the typing judgment of `qfs`.
               Even if we would ask for the F* typing judgement of `qfs`,
               it could be just a token---not helpful.
-              Maybe there is a way to recover by normalizing a bit `hd`?
+              Maybe there is a way to recover by normalizing a bit `hd`? See: recover_type_of_arrow
           QA: How would this work with the logical relation? **) 
     // assert (forall t. tot_typing gfs (Tv_App hd (a, _)) qty ==> 
     //           (exists t'. tot_typing gfs a t' /\ tot_typing gfs hd (Tv_Arrow t' qty)));
     // assert (forall t. tot_typing gfs (Tv_App hd (a, _)) qty ==> 
     //           (forall t'. tot_typing gfs hd (Tv_Arrow t' qty) ==> tot_typing gfs a t'));
-    let (| _, sa_ty, sa_tyj |) = unverified_exp_translation gfs gstlc vars_mapping a in
-    let (| _, shd_ty, shd_tyj |) = unverified_exp_translation gfs gstlc vars_mapping hd in
+    let (| _, sa_ty, sa_tyj |) = exp_translation gfs gstlc vars_mapping a in
+    let (| _, shd_ty, shd_tyj |) = exp_translation gfs gstlc vars_mapping hd in
     match shd_ty with
     | STLC.TArr arg res -> 
       if arg = sa_ty then (| _, res, STLC.TyApp shd_tyj sa_tyj |)
@@ -146,9 +146,10 @@ let rec unverified_exp_translation
 
   | Tv_Abs bin body -> begin
     let gfs' = extend_env gfs bin.uniq bin.sort in
-    let bin_ty : STLC.typ = unverified_typ_translation gfs bin.sort in
+    let bin_ty : STLC.typ = typ_translation gfs bin.sort in
+    (* TODO: don't I have to prove termination here? is it hidden in extend_env_mapping? *)
     let (| gstlc', vars_mapping' |) = extend_env_mapping gstlc vars_mapping bin bin_ty in
-    let (| _, _, body_tyj |) = unverified_exp_translation gfs' gstlc' vars_mapping' body in
+    let (| _, _, body_tyj |) = exp_translation gfs' gstlc' vars_mapping' body in
     (| _, _, STLC.TyLam #gstlc bin_ty body_tyj |) 
   end
 
@@ -156,6 +157,17 @@ let rec unverified_exp_translation
     if (x < 0) then fail ("not supporting ints, only nats") else
     let (| e, tyj |) = make_stlc_nat x in
     (| e, STLC.TNat, tyj |)
+
+  // | Tv_Let    : recf:bool -> attrs:(list term) -> b:simple_binder -> def:term -> body:term -> named_term_view
+  // | Tv_Let recf attr bin def body -> begin
+  //   let gfs' = extend_env gfs bin.uniq bin.sort in
+  //   let bin_ty : STLC.typ = typ_translation gfs bin.sort in
+  //   let (| _, def_ty, def_tyj |) = exp_translation gfs gstlc vars_mapping def in
+  //   if def_ty <> bin_ty then fail ("converting let failed because definition type mismatch") else
+  //   let (| gstlc', vars_mapping' |) = extend_env_mapping gstlc vars_mapping bin bin_ty in
+  //   let (| _, body_ty, body_tyj |) = exp_translation gfs' gstlc' vars_mapping' body in
+  //   (| _, body_ty, STLC.TyApp #gstlc #_ #_ #bin_ty #body_ty (STLC.TyLam #gstlc bin_ty body_tyj) def_tyj |)
+  // end
 
   | Tv_Unknown -> fail ("an underscore was found in the term")
   | Tv_Unsupp -> fail ("unsupported by F* terms")
@@ -165,10 +177,10 @@ let rec unverified_exp_translation
 let mk_stlc_typing (g qexp qtyp:term) =
   mk_app (`STLC.typing) [(g, Q_Explicit); (qexp, Q_Explicit); (qtyp, Q_Explicit)]	
 
-let comp_exp (nm:string) (qfs:term) : dsl_tac_t = fun g ->
+let def_translation (nm:string) (qfs:term) : dsl_tac_t = fun g ->
   let qfs = norm_term_env g [delta] qfs in
   let (| exp, typ, tyj |) : open_stlc_term STLC.empty =
-    unverified_exp_translation g STLC.empty (fun _ _ -> None) qfs in
+    exp_translation g STLC.empty (fun _ _ -> None) qfs in
   let qexp = quote exp in
   type_dynamically g qexp (`STLC.exp);
   let qtyp = quote typ in
@@ -191,7 +203,7 @@ let stlc_sem (#e:STLC.exp) (#t:STLC.typ) (ht:STLC.typing STLC.empty e t) : STLC.
   STLC.elab_exp ht' STLC.vempty
 
 let src1 : nat = 4
-%splice_t[tgt1;tgt1_typ;tgt1_tyj] (comp_exp "tgt1" (`src1))
+%splice_t[tgt1;tgt1_typ;tgt1_tyj] (def_translation "tgt1" (`src1))
 let _ = 
   assert (tgt1 == STLC.ESucc (STLC.ESucc (STLC.ESucc (STLC.ESucc STLC.EZero))));
   assert (stlc_sem tgt1_tyj == src1)
@@ -203,9 +215,18 @@ let _ =
 //   assert (tgt2 == STLC.EZero)
 
 let src3 : nat -> nat -> nat = fun x y -> x
-%splice_t[tgt3;tgt3_typ;tgt3_tyj] (comp_exp "tgt3" (`src3))
+%splice_t[tgt3;tgt3_typ;tgt3_tyj] (def_translation "tgt3" (`src3))
 
-let test () =
+let test3 () =
   assert (tgt3_typ == STLC.TArr STLC.TNat (STLC.TArr STLC.TNat STLC.TNat));
   assert (tgt3 == STLC.ELam STLC.TNat (STLC.ELam STLC.TNat (STLC.EVar 1)));
   assert (forall x y. (stlc_sem tgt3_tyj) x y == x /\ (stlc_sem tgt3_tyj) x y == src3 x y)
+
+let src4 : nat -> (nat -> nat) -> nat = fun x f -> let y = f x in y
+%splice_t[tgt4;tgt4_typ;tgt4_tyj] (def_translation "tgt4" (`src4))
+
+let test4 () =
+  assert (tgt4_typ == STLC.TArr STLC.TNat (STLC.TArr (STLC.TArr STLC.TNat STLC.TNat) STLC.TNat));
+  assert (tgt4 == STLC.ELam STLC.TNat
+                   (STLC.ELam (STLC.TArr STLC.TNat STLC.TNat) (STLC.EApp (STLC.EVar 0) (STLC.EVar 1))))
+  // assert (forall x. (stlc_sem tgt4_tyj) x == x /\ (stlc_sem tgt4_tyj) x == src4 x)
